5 cases left

src/rocq/Semantics/Operations/Select.v
@@ -8,6 +8,27 @@ From Vellvm Require Import
 Section Select.
   Context {Pa : Params}.
 
+  (* Pointwise select over vectors; top-level (rather than a local [fix])
+     so that proofs can state lemmas about it. *)
+  Fixpoint select_loop (conds xs ys : list dvalue) : EOU (list dvalue) :=
+    match conds, xs, ys with
+    | [], [], [] => ret []
+    | (c::conds), (x::xs), (y::ys) =>
+        selected <- match c with
+                   | DVALUE_Poison t =>
+                       (* TODO: Should be the type of the result of the select... *)
+                       ret (DVALUE_Poison t)
+                   | DVALUE_I 1 i =>
+                       if (@Integers.unsigned 1 i =? 1)%Z
+                       then ret x
+                       else ret y
+                   | _ => raise_error "eval_select: ill-typed select, condition in vector was not poison or i1."
+                   end;;
+        rest <- select_loop conds xs ys;;
+        ret (selected :: rest)
+    | _, _, _ => raise_error "eval_select: ill-typed vector select, length mismatch."
+    end.
+
   Definition eval_select
     (cnd : dvalue) (v1 v2 : dvalue) : EOU dvalue
     := match cnd with
@@ -19,24 +40,6 @@ Section Select.
            then ret v1
            else ret v2
        | DVALUE_Vector _ conds =>
-           let fix loop conds xs ys : EOU (list dvalue) :=
-             match conds, xs, ys with
-             | [], [], [] => ret []
-             | (c::conds), (x::xs), (y::ys) =>
-                 selected <- match c with
-                            | DVALUE_Poison t =>
-                                (* TODO: Should be the type of the result of the select... *)
-                                ret (DVALUE_Poison t)
-                            | DVALUE_I 1 i =>
-                                if (@Integers.unsigned 1 i =? 1)%Z
-                                then ret x
-                                else ret y
-                            | _ => raise_error "eval_select: ill-typed select, condition in vector was not poison or i1."
-                            end;;
-                 rest <- loop conds xs ys;;
-                 ret (selected :: rest)
-             | _, _, _ => raise_error "eval_select: ill-typed vector select, length mismatch."
-             end in
            match v1, v2 with
            | DVALUE_Poison t, _ =>
                (* TODO: Should we make sure t is a vector type...? *)
@@ -45,7 +48,7 @@ Section Select.
                (* TODO: Should we make sure t is a vector type...? *)
                ret (DVALUE_Poison t)
            | DVALUE_Vector t xs, DVALUE_Vector _ ys =>
-               selected <- loop conds xs ys;;
+               selected <- select_loop conds xs ys;;
                ret (DVALUE_Vector t selected)
            | _, _ => raise_error "eval_select: ill-typed vector select, non-vector arguments"
            end
